CCsub_RuntimeInversion.v
@@ -1,11 +1,96 @@
 Require Import Coq.Program.Equality.
+Require Import LibTactics.
+
 Require Import CCsub_Subcapt.
 Require Import CCsub_Subtyping.
 Require Import CCsub_Typing.
 Require Import CCsub_Substitution.
 Require Import CCsub_Red.
+Require Import CCsub_Precise.
 
 Hint Constructors store_typing eval_typing state_typing : core.
+
+(************************************************************************ *)
+(** ** Properties of values *)
+
+Lemma capture_prediction : forall Γ v E C R S,
+  value (v, E) ->
+  typing Γ S v (C # R) ->
+  subcapt Γ S (exp_cv v) C.
+Proof with subst; simpl; eauto.
+  intros * Value Typ.
+  forwards (WfS & WfCtx & Expr & WfTyp): typing_regular Typ.
+  eremember (C # R) as T.
+  assert (sub Γ S T (C # R)) by (rewrite HeqT; apply sub_reflexivity; eauto* ).
+  clear HeqT.
+  generalize dependent R.
+  generalize dependent C.
+  induction Typ; intros C0 R0 Sub; cbn [exp_cv]; try solve [ inversion Value ].
+  - inversion WfTyp; subst.
+    inversion Sub...
+  - inversion WfTyp; subst.
+    inversion Sub...
+  - apply subcapt_bot.
+    enough (WfC0R0 : wf_typ Γ S (C0 # R0)) by (inversion WfC0R0; auto).
+    applys sub_regular Sub.
+    apply sub_regular in Sub.
+    destruct Sub as [_ [_ [_ WF_C0]]].
+    inversion WF_C0; subst...
+  - forwards: IHTyp...
+    apply (sub_transitivity T)...
+Qed.
+
+Lemma values_have_precise_captures : forall Γ v E C R S,
+  value (v, E) ->
+  typing Γ S v (C # R) ->
+  exists U, typing Γ S v (exp_cv v # U) /\
+            sub Γ S (exp_cv v # U) (C # R).
+Proof with simpl; eauto*.
+  intros * Value Typ.
+  assert (wf_cse Γ S (exp_cv v)) by eauto using typing_cv.
+  assert (wf_ctx Γ S) by applys typing_regular Typ.
+  assert (wf_store_ctx S) by applys typing_regular Typ.
+  induction Typ; try solve [inversion Value; subst].
+  - Case "typing_abs".
+    exists (∀ (C0 # R0) T1).
+    split...
+    eapply sub_reflexivity...
+    constructor...
+    + econstructor...
+      intros x xIn.
+      rename select (forall x : atom, x ∉ L -> typing _ _ (open_ve _ _ _)  _) into IH.
+      forwards Typ: (IH x xIn).
+      applys typing_regular Typ.
+    + econstructor.
+      1: eapply type_from_wf_typ...
+      intros x xIn.
+      rename select (forall x : atom, x ∉ L -> typing _ _ (open_ve _ _ _)  _) into IH.
+      forwards Typ: (IH x xIn).
+      eapply type_from_wf_typ...
+  - Case "typing_tabs".
+    exists (∀ [V] T1).
+    split...
+    eapply sub_reflexivity...
+    constructor...
+    + econstructor...
+      intros x xIn.
+      rename select (forall x : atom, x ∉ L -> typing _ _ (open_te _ _) _) into IH.
+      forwards Typ: (IH x xIn).
+      applys typing_regular Typ.
+    + econstructor...
+      intros x xIn.
+      rename select (forall x : atom, x ∉ L -> typing _ _ (open_te _ _) _) into IH.
+      forwards Typ: (IH x xIn).
+      eapply type_from_wf_typ...
+  - Case "typing_box".
+    exists (□ (C0 # R0)).
+    split...
+    apply sub_reflexivity...
+  - Case "typing_sub".
+    forwards (U & HtypU & HsubS): IHTyp...
+    exists U. split...
+    eauto using (sub_transitivity R0).
+Qed.
 
 Definition no_type_bindings (Γ : ctx) : Prop :=
   forall X U, ~ binds X (bind_sub U) Γ.
@@ -113,6 +198,14 @@ Proof with eauto*.
   rewrite IHStoreTyp...
 Qed.
 
+Lemma env_well_typed_preserves_dom : forall S E Γ,
+  env_well_typed S E Γ ->
+  dom E = dom Γ.
+Proof with eauto*.
+  intros * EnvTyp. dependent induction EnvTyp...
+  simpl. rewrite IHEnvTyp...
+Qed.
+
 Lemma typed_store_ctx_wf : forall S SS,
   store_typing SS S ->
   wf_store_ctx S.
@@ -151,6 +244,9 @@ Lemma env_well_typed_ctx_wf : forall Γ S E,
   wf_ctx Γ S.
 Proof with eauto.
   intros. dependent induction H...
+  constructor...
+  eapply env_well_typed_store_ctx_wf in H.
+  eapply wf_typ_from_wf_store_ctx...
 Qed.
 
 Lemma env_well_typed_weaken_store : forall Γ S1 S2 S3 E,
@@ -239,22 +335,22 @@ Lemma env_typing_equivalent : forall S E Γ x,
 Proof with eauto.
   intros * EnvTyp. dependent induction EnvTyp; split; intros.
   1,2: destruct H0 as [? [? Binds]]; inversion Binds.
-  - destruct H2 as [l0 [T Binds]].
+  - destruct H1 as [l0 [T Binds]].
     binds_cases Binds; subst.
     + assert (exists l T, binds x (T, l) E) by (exists l0, T; eauto).
-      destruct ((proj1 IHEnvTyp) H3) as [C0 [R0 Binds]].
+      destruct ((proj1 IHEnvTyp) H2) as [C0 [R0 Binds]].
       exists C0, R0.
       apply binds_tail with (F := [(x0, bind_typ (C # R))]) in Binds; simpl in *...
-    + inversion H4; subst.
+    + inversion H3; subst.
       exists C, R.
       apply binds_head, binds_singleton.
-  - destruct H2 as [C0 [R0 Binds]].
+  - destruct H1 as [C0 [R0 Binds]].
     binds_cases Binds; subst.
     + assert (exists C R, binds x (bind_typ (C # R)) Γ) by (exists C0, R0; eauto).
-      destruct ((proj2 IHEnvTyp) H3) as [l0 [T Binds]].
+      destruct ((proj2 IHEnvTyp) H2) as [l0 [T Binds]].
       exists l0, T.
       apply binds_tail with (F := [(x0, (C # R, l))]) in Binds; simpl in *...
-    + inversion H4; subst.
+    + inversion H3; subst.
       exists l, (C # R).
       apply binds_head, binds_singleton.
 Qed.
@@ -262,38 +358,166 @@ Qed.
 Lemma env_typing_inversion : forall S E Γ x C R l,
   env_well_typed S E Γ ->
   binds x (C # R, l) E ->
-  Store.binds l (C # R) S /\ binds x (bind_typ (C # R)) Γ /\ wf_typ Γ S (C # R).
+  Store.binds l (C # R) S /\ binds x (bind_typ (C # R)) Γ /\ wf_typ nil S (C # R).
 Proof with eauto.
   intros * EnvTyp Binds.
   dependent induction EnvTyp.
   { inversion Binds. }
   assert (WfCtx : wf_ctx Γ S) by (eapply env_well_typed_ctx_wf; eauto).
   binds_cases Binds; subst.
-  - destruct (IHEnvTyp H2) as [StoreBinds [Binds Wf]].
+  - destruct (IHEnvTyp H1) as [StoreBinds [Binds Wf]].
     repeat split...
-    rewrite_nil_concat.
-    eapply wf_typ_weakening...
-    constructor...
-  - inversion H4; subst.
+  - inversion H3; subst.
     repeat split...
-    rewrite_nil_concat.
-    eapply wf_typ_weakening...
-    constructor...
+    assert (WfS : wf_store_ctx S) by applys env_well_typed_store_ctx_wf EnvTyp.
+    eapply wf_typ_from_wf_store_ctx_nil...
 Qed.
 
-(* Lemma stores_preserves_typing : forall SS Γ S E E' (x : atom) l v C R T, *)
-(*   store_typing SS S -> *)
-(*   env_well_typed S E Γ -> *)
-(*   binds x (T, l) E -> *)
-(*   stores l (v, E') SS -> *)
-(*   typing Γ S x (C # R) -> *)
-(*   exists D Q, typing Γ S v (exp_cv v # Q) *)
-(*          /\ binds x (bind_typ (D # Q)) Γ *)
-(*          /\ subcapt Γ S (exp_cv v) D *)
-(*          /\ sub Γ S Q R. *)
+Lemma prec_typing_weakening_store : forall Γ e T S1 S2 S3,
+  prec_typing Γ (S1 ++ S3) e T ->
+  wf_store_ctx (S1 ++ S2 ++ S3) ->
+  prec_typing Γ (S1 ++ S2 ++ S3) e T.
+Proof with eauto using
+  wf_typ_weakening_store,
+  wf_cse_weakening_store,
+  wf_ctx_weakening_store,
+  sub_weakening_store,
+  subcapt_weakening_store.
+  intros * Typ. remember (S1 ++ S3).
+  generalize dependent S1.
+  induction Typ; intros S1 EQ Ok; subst...
+  - pick fresh x and apply prec_typing_abs...
+  - pick fresh x and apply prec_typing_let...
+  - pick fresh x and apply prec_typing_tabs...
+Qed.
+
+Lemma prec_store_typing_inversion : forall SS S l v E U,
+  prec_store_typing SS S ->
+  Store.binds l U S ->
+  stores l (v, E) SS ->
+  exists Γ, (prec_typing Γ S v U /\ env_well_typed S E Γ /\ wf_typ nil S U /\ value(v, E)).
+Proof with eauto using prec_typing_weakening_store, env_well_typed_weaken_store, wf_typ_weakening_store.
+  intros * PStoreTyp lBindsU lBindsv.
+  dependent induction PStoreTyp.
+  inversion lBindsU.
+  assert (StoreTyp : store_typing SS S) by (eapply prec_store_typing_implies_store_typing; eauto).
+  assert (WfStore : wf_store_ctx S) by applys typed_store_ctx_wf StoreTyp.
+  rewrite_env ([(l0, (C # R))] ++ S) in lBindsU.
+  Store.binds_cases lBindsU; subst.
+  - rewrite_env ([(l0, store (v0, E0))] ++ SS) in lBindsv.
+    unfold stores in lBindsv. Store.binds_cases lBindsv...
+    + destruct (IHPStoreTyp H4 H5) as [Γ0 [Typ [EnvTyp [WfU Val]]]].
+      assert (wf_store_ctx ([(l0, C # R)] ++ S)) by (constructor; eauto).
+      exists Γ0; rewrite_env (nil ++ [(l0, C # R)] ++ S)...
+      repeat split...
+    + simpl in Fr; flsetdec.
+  - rewrite_env ([(l, store (v0, E0))] ++ SS) in lBindsv.
+    unfold stores in lBindsv. Store.binds_cases lBindsv...
+    + simpl in Fr; flsetdec.
+    + inversion H6; subst.
+      assert (wf_store_ctx ([(l, C # R)] ++ S)) by (constructor; eauto).
+      exists Γ; rewrite_env (nil ++ [(l, C # R)] ++ S).
+      repeat split; auto.
+      apply prec_typing_weakening_store...
+      apply env_well_typed_weaken_store...
+      apply wf_typ_weakening_store...
+Qed.
+
+Lemma val_env : forall E v,
+  value (v, E) ->
+  fv_ve v = dom E.
+Proof with eauto.
+  intros * Value.
+  dependent induction Value; simpl; eauto.
+Qed.
+
+Lemma subcapt_union_means_subcapt_individual : forall Γ S C1 C2 D,
+  subcapt Γ S (C1 `u` C2) D ->
+  subcapt Γ S C1 D /\ subcapt Γ S C2 D.
+Proof with eauto.
+  intros * Subcapt.
+  dependent induction Subcapt; simpl in *; eauto.
+  - inverts H0.
+    split; constructor...
+  - destruct (IHSubcapt C1 C2 eq_refl).
+    split; constructor...
+  - destruct (IHSubcapt C1 C2 eq_refl).
+    split; apply subcapt_join_inr...
+Qed.
+
+(* Lemma exp_cv_sub_wf_empty : forall Γ S C e, *)
+(*   wf_cse nil S C -> *)
+(*   subcapt Γ S (exp_cv e) C -> *)
+(*   fv_ve e = {}A. *)
 (* Proof with eauto. *)
-(*   intros * StoreTyp EnvTyp Binds Stores. *)
-(*   revert C R. *)
-(*   dependent induction StoreTyp. *)
-(*   { inversion Stores. } *)
-(*   intros C0 R0 xTyp. *)
+(*   intros * WfC Sub. *)
+(*   assert (fv_ve e = cse_fvars (exp_cv e)). { *)
+(*     induction e; simpl in *; eauto. *)
+(*     - destruct v... *)
+(*     - destruct v; simpl in *; destruct v0... *)
+(*     - destruct (subcapt_union_means_subcapt_individual _ _ _ _ _ Sub)... *)
+(*       rewrite <- IHe1, IHe2... *)
+(*     - destruct v... *)
+(*     - destruct v... *)
+(*       admit. *)
+(*     -  *)
+(*   } *)
+
+
+(* Lemma stores_preserves_typing : forall S Γ x v C P, *)
+(*   S ∷ Γ -> *)
+(*   stores S x v -> *)
+(*   Γ ⊢ x : (C # P) -> *)
+(*   exists D Q, Γ ⊢ v : (exp_cv v # Q) *)
+(*          /\ binds x (bind_typ (D # Q)) Γ *)
+(*          /\ Γ ⊢ₛ (exp_cv v) <: D *)
+(*          /\ Γ ⊢ Q <: P. *)
+
+Lemma prec_typing_strengthen_var : forall Γ S (x x0 : atom) C R C1 R1,
+  prec_typing ((x0, bind_typ (C1 # R1)) :: Γ) S x (C # R) ->
+  x <> x0 ->
+  prec_typing Γ S x (C # R).
+Proof with eauto.
+  intros * PTyp xNeq.
+  dependent induction PTyp; simpl; eauto.
+  rewrite_env ([(x0, bind_typ (C1 # R1))] ++ Γ) in H0.
+  binds_cases H0; subst.
+  eapply prec_typing_var...
+  inverts H...
+Qed.
+
+Lemma prec_typing_values_have_precise_captures : forall Γ S v E C R,
+  value (v, E) ->
+  prec_typing Γ S v (C # R) ->
+  C = exp_cv v.
+Proof with eauto.
+  intros * Value PTyp.
+  dependent induction PTyp; simpl in *; try solve [inversion Value; subst]...
+Qed.
+
+Lemma stores_preserves_typing : forall SS Γ S E E0 (x : atom) l v C R C0 R0,
+  prec_store_typing SS S ->
+  env_well_typed S E Γ ->
+  binds x (C0 # R0, l) E ->
+  stores l (v, E0) SS ->
+  prec_typing Γ S x (C # R) ->
+  exists Γ0,
+    prec_typing Γ0 S v (exp_cv v # R) /\
+    env_well_typed S E0 Γ0.
+Proof with eauto.
+  intros * PStoreTyp EnvTyp Binds Stores xPTyp.
+  assert (StoreTyp : store_typing SS S) by (eapply prec_store_typing_implies_store_typing; eauto).
+  assert (xTyp : typing Γ S x (C # R)) by (eapply prec_typing_implies_typing; eauto).
+  destruct (typing_var_implies_binds_typ _ _ _ _ _ xTyp) as [D [Q [Binds2 [Subcapt [Wf [Sub Pure]]]]]].
+  dependent induction xPTyp; simpl in *...
+  epose proof (binds_unique _ _ _ _ H0 Binds2).
+  inverts H1.
+  epose proof (env_typing_inversion _ _ _ _ _ _ _ EnvTyp Binds).
+  destruct H1 as [lBinds2 [Binds3 _]].
+  epose proof (binds_unique _ _ _ _ H0 Binds3).
+  inverts H1.
+  epose proof (prec_store_typing_inversion _ _ _ _ _ _ PStoreTyp lBinds2 Stores).
+  destruct H1 as [Γ0 [PTyp [EnvTyp0 [WfU Val]]]].
+  epose proof (prec_typing_values_have_precise_captures _ _ _ _ _ _ Val PTyp); subst.
+  exists Γ0...
+Qed.
